src/prop/FutureCertify.v
@@ -89,7 +89,7 @@ Module FutureCertify.
           { i. econs; eauto. }
         }
       }
-      { eapply mapping_map_lt_collapsable_unwritable. eapply ident_map_lt. }
+      { eapply mapping_map_lt_iff_collapsable_unwritable. eapply ident_map_lt. }
       { eapply ident_map_timemap. }
       { eapply Memory.max_concrete_timemap_spec; eauto.
         eapply Memory.cap_closed_timemap; eauto. }
