src/prop/JoinedView.v
@@ -1039,12 +1039,11 @@ Module JSim.
         (ThreadEvent.write loc from to val released_src ord)
         (ThreadEvent.write loc from to val released_tgt ord)
   | sim_event_write_na
-      loc msgs from to val released_src released_tgt ord
-      (RELEASED: View.opt_le released_src released_tgt)
+      loc msgs from to val ord
     :
       sim_event
-        (ThreadEvent.write_na loc msgs from to val released_src ord)
-        (ThreadEvent.write_na loc msgs from to val released_tgt ord)
+        (ThreadEvent.write_na loc msgs from to val ord)
+        (ThreadEvent.write_na loc msgs from to val ord)
   | sim_event_update
       loc tsr tsw valr valw releasedr_src releasedr_tgt releasedw_src releasedw_tgt ordr ordw
       (RELEASEDR: View.opt_le releasedr_src releasedr_tgt)
@@ -3002,7 +3001,7 @@ Module JSim.
       + hexploit sim_local_write_na_step; eauto.
         { refl. }
         i. des.
-        eexists (ThreadEvent.write_na _ _ _ _ _ _ _). esplits.
+        eexists (ThreadEvent.write_na _ _ _ _ _ _). esplits.
         * econs.
           { econs 2; eauto. econs; eauto. }
           { ss. }
@@ -3011,7 +3010,7 @@ Module JSim.
           { ss. }
           { ss. }
         * ss.
-        * econs. refl.
+        * econs.
 
       + hexploit sim_local_racy_read; eauto.
         { refl. }
